Now [OStateIfc] is a typeclass

src/Ex/Mesi/Mesi.v
@@ -13,13 +13,13 @@ Local Open Scope fmap.
 
 Section Template.
   Variable (dtr: DTree).
-  Context {ifc: OStateIfc}.
+  Context `{oifc: OStateIfc}.
   Variables (ridx msgId: IdxT).
 
   (* Heads-up: [cidx] is not the index of itself, but of a child. *)
   Definition immDownRule (cidx: IdxT)
-             (prec: OPrec ifc)
-             (trs: OState ifc -> Msg -> OState ifc * Msg): Rule ifc :=
+             (prec: OPrec)
+             (trs: OState -> Msg -> OState * Msg): Rule :=
     rule[ridx]
     :requires (MsgsFrom [rqUpFrom cidx] /\ MsgIdsFrom [msgId] /\
                RqAccepting /\ UpLockFree /\ DownLockFree /\ prec)
@@ -29,8 +29,8 @@ Section Template.
                      (ost, st.orq, [(downTo cidx, out)]))).
 
   Definition immUpRule (oidx: IdxT)
-             (prec: OPrec ifc)
-             (trs: OState ifc -> Msg -> OState ifc * Msg): Rule ifc :=
+             (prec: OPrec)
+             (trs: OState -> Msg -> OState * Msg): Rule :=
     rule[ridx]
     :requires (MsgsFrom [downTo oidx] /\ MsgIdsFrom [msgId] /\
                RqAccepting /\ DownLockFree /\ prec)
@@ -40,8 +40,8 @@ Section Template.
                      (ost, st.orq, [(rqUpFrom oidx, out)]))).
 
   Definition rqUpUpRule (cidx oidx: IdxT)
-             (prec: OPrec ifc)
-             (trs: OState ifc -> Msg -> Msg): Rule ifc :=
+             (prec: OPrec)
+             (trs: OState -> Msg -> Msg): Rule :=
     rule[ridx]
     :requires (MsgsFrom [rqUpFrom cidx] /\ MsgIdsFrom [msgId] /\
                RqAccepting /\ UpLockFree /\ prec)
@@ -52,8 +52,8 @@ Section Template.
                       [(rqUpFrom oidx, trs (st.ost) msg)]))).
 
   Definition rqUpUpRuleS (oidx: IdxT)
-             (prec: OPrec ifc)
-             (trs: OState ifc -> Msg): Rule ifc :=
+             (prec: OPrec)
+             (trs: OState -> Msg): Rule :=
     rule[ridx]
     :requires (MsgsFrom nil /\ RqAccepting /\ UpLockFree /\ prec)
     :transition
@@ -64,8 +64,8 @@ Section Template.
 
   (** * FIXME: need to know children indices from [trs] are sound. *)
   Definition rqUpDownRule (cidx oidx: IdxT)
-             (prec: OPrec ifc)
-             (trs: OState ifc -> Msg -> list IdxT * Msg): Rule ifc :=
+             (prec: OPrec)
+             (trs: OState -> Msg -> list IdxT * Msg): Rule :=
     rule[ridx]
     :requires (MsgsFrom [rqUpFrom cidx] /\ MsgIdsFrom [msgId] /\
                RqAccepting /\ UpLockFree /\ DownLockFree /\ prec)
@@ -78,8 +78,8 @@ Section Template.
 
   (** * FIXME: need to know children indices from [trs] are sound. *)
   Definition rqDownDownRule (oidx: IdxT)
-             (prec: OPrec ifc)
-             (trs: OState ifc -> Msg -> list IdxT * Msg): Rule ifc :=
+             (prec: OPrec)
+             (trs: OState -> Msg -> list IdxT * Msg): Rule :=
     rule[ridx]
     :requires (MsgsFrom [downTo oidx] /\ MsgIdsFrom [msgId] /\
                RqAccepting /\ DownLockFree /\ prec)
@@ -91,12 +91,12 @@ Section Template.
                       map (fun cidx => (downTo cidx, msg)) cinds))).
 
   Definition rsDownDownRule (rqId: IdxT)
-             (prec: OPrec ifc)
-             (trs: OState ifc ->
+             (prec: OPrec)
+             (trs: OState ->
                    Msg (* an incoming message *) ->
                    Msg (* the original request *) ->
                    IdxT (* response back to *) ->
-                   OState ifc * Msg) :=
+                   OState * Msg) :=
     rule[ridx]
     :requires (MsgsFromORq upRq /\ MsgIdsFrom [msgId] /\ UpLockMsgId MRq rqId /\
                RsAccepting /\ DownLockFree /\ prec)
@@ -108,11 +108,11 @@ Section Template.
                      (ost, removeRq (st.orq) upRq, [(rsbTo, out)]))).
 
   Definition rsDownDownRuleS (rqId: IdxT)
-             (prec: OPrec ifc)
-             (trs: OState ifc ->
+             (prec: OPrec)
+             (trs: OState ->
                    Msg (* an incoming message *) ->
                    Msg (* the original request *) ->
-                   OState ifc) :=
+                   OState) :=
     rule[ridx]
     :requires (MsgsFromORq upRq /\ MsgIdsFrom [msgId] /\ UpLockMsgId MRq rqId /\
                RsAccepting /\ DownLockFree /\ prec)
@@ -125,13 +125,13 @@ Section Template.
                       nil))).
 
   Definition rsUpDownRule (rqId: IdxT)
-             (prec: OPrec ifc)
-             (trs: OState ifc ->
+             (prec: OPrec)
+             (trs: OState ->
                    list (Id Msg) (* incoming messages *) ->
                    Msg (* the original request *) ->
                    list IdxT (* responses from *) ->
                    IdxT (* response back to *) ->
-                   OState ifc * Msg) :=
+                   OState * Msg) :=
     rule[ridx]
     :requires (MsgsFromORq downRq /\ MsgIdFromEach msgId /\
                DownLockMsgId MRq rqId /\ RsAccepting /\ prec)
@@ -145,13 +145,13 @@ Section Template.
                       [(rsbTo, out)]))).
 
   Definition rsUpUpRule (rqId: IdxT)
-             (prec: OPrec ifc)
-             (trs: OState ifc ->
+             (prec: OPrec)
+             (trs: OState ->
                    list (Id Msg) (* incoming messages *) ->
                    Msg (* the original request *) ->
                    list IdxT (* responses from *) ->
                    IdxT (* response back to *) ->
-                   OState ifc * Msg) :=
+                   OState * Msg) :=
     rule[ridx]
     :requires (MsgsFromORq downRq /\ MsgIdFromEach msgId /\
                DownLockMsgId MRq rqId /\ RsAccepting /\ prec)
@@ -166,8 +166,8 @@ Section Template.
 
   (** * FIXME: need to know children indices from [trs] are sound. *)
   Definition rsDownRqDownRule (rqId: IdxT)
-             (prec: OPrec ifc)
-             (trs: OState ifc -> Msg -> list IdxT * Msg) :=
+             (prec: OPrec)
+             (trs: OState -> Msg -> list IdxT * Msg) :=
     rule[ridx]
     :requires (MsgsFromORq upRq /\ MsgIdsFrom [msgId] /\
                UpLockMsgId MRq rqId /\
@@ -280,13 +280,13 @@ Section System.
 
   End Directory.
 
-  Definition ImplOStateIfc: OStateIfc :=
+  Instance ImplOStateIfc: OStateIfc :=
     {| ost_ty := [nat:Type; MESI:Type; DirT:Type]%vector |}.
 
-  Definition implOStateInit: OState ImplOStateIfc :=
+  Definition implOStateInit: OState :=
     (0, (mesiS, (dirInit, tt))).
   
-  Definition implOStatesInit: OStates ImplOStateIfc :=
+  Definition implOStatesInit: OStates :=
     fold_left (fun m i => m +[i <- implOStateInit])
               (cifc.(c_l1_indices) ++ cifc.(c_li_indices)) [].
 
@@ -295,7 +295,7 @@ Section System.
 
   (** A core idea: a "summary" status in each object *)
 
-  Definition summaryOf (ost: OState ImplOStateIfc): MESI :=
+  Definition summaryOf (ost: OState): MESI :=
     if Compare_dec.le_gt_dec mesiS ost#[implStatusIdx]
     then ost#[implStatusIdx]
     else ost#[implDirIdx].(dir_st).
@@ -305,43 +305,37 @@ Section System.
 
     Section GetTrs.
 
-      Definition l1GetSImm: Rule ImplOStateIfc :=
+      Definition l1GetSImm: Rule :=
         rule.immd[cidx~>0~>0]
         :accepts mesiRqS
         :from cidx
-        :requires
-           (fun (ost: OState ImplOStateIfc) orq mins =>
-               mesiS <= ost#[implStatusIdx])
+        :requires (fun ost orq mins => mesiS <= ost#[implStatusIdx])
         :transition
-           (fun (ost: OState ImplOStateIfc) _ =>
+           (fun ost _ =>
               (ost, {| msg_id := mesiRsS;
                        msg_type := MRs;
                        msg_value := VNat (ost#[implValueIdx])
                     |})).
 
-      Definition liGetSImmS: Rule ImplOStateIfc :=
+      Definition liGetSImmS: Rule :=
         rule.immd[cidx~>0~>0~>0]
         :accepts mesiRqS
         :from cidx
-        :requires
-           (fun (ost: OState ImplOStateIfc) orq mins =>
-               ost#[implStatusIdx] = mesiS)
+        :requires (fun ost orq mins => ost#[implStatusIdx] = mesiS)
         :transition
-           (fun (ost: OState ImplOStateIfc) _ =>
+           (fun ost _ =>
               (ost, {| msg_id := mesiRsS;
                        msg_type := MRs;
                        msg_value := VNat (ost#[implValueIdx])
                     |})).
 
-      Definition liGetSImmME: Rule ImplOStateIfc :=
+      Definition liGetSImmME: Rule :=
         rule.immd[cidx~>0~>0~>1]
         :accepts mesiRqS
         :from cidx
-        :requires
-           (fun (ost: OState ImplOStateIfc) orq mins =>
-              mesiE <= ost#[implStatusIdx])
+        :requires (fun ost orq mins => mesiE <= ost#[implStatusIdx])
         :transition
-           (fun (ost: OState ImplOStateIfc) _ =>
+           (fun ost _ =>
               (ost +#[implStatusIdx <- mesiS]
                    +#[implDirIdx <- setDirS [cidx]],
                {| msg_id := mesiRsS;
@@ -355,28 +349,26 @@ Section System.
        *)
 
       (* commonly used *)
-      Definition getSRqUpUp: Rule ImplOStateIfc :=
+      Definition getSRqUpUp: Rule :=
         rule.rquu[cidx~>0~>1]
         :accepts mesiRqS
         :from cidx
         :me oidx
-        :requires
-           (fun (ost: OState ImplOStateIfc) orq mins =>
-              summaryOf ost = mesiI)
+        :requires (fun ost orq mins => summaryOf ost = mesiI)
         :transition
-           (fun (ost: OState ImplOStateIfc) msg =>
+           (fun ost msg =>
               {| msg_id := mesiRqS;
                  msg_type := MRq;
                  msg_value := VUnit |}).
 
       (** * FIXME: how to get "n"? *)
-      Definition l1GetSRsDownDownS: Rule ImplOStateIfc :=
+      Definition l1GetSRsDownDownS: Rule :=
         rule.rsdd[0~>2~>0]
         :accepts mesiRsS
         :holding mesiRqS
         :requires FirstNatMsg
         :transition
-           (fun (ost: OState ImplOStateIfc) min rq rsbTo =>
+           (fun ost min rq rsbTo =>
               (* n <-- getNatMsg; *)
               let n := O in
               (ost +#[implValueIdx <- n]
@@ -385,13 +377,13 @@ Section System.
                   msg_type := MRs;
                   msg_value := VNat n |})).
 
-      Definition l1GetSRsDownDownE: Rule ImplOStateIfc :=
+      Definition l1GetSRsDownDownE: Rule :=
         rule.rsdd[0~>2~>1]
         :accepts mesiRsE
         :holding mesiRqS
         :requires FirstNatMsg
         :transition
-           (fun (ost: OState ImplOStateIfc) min rq rsbTo =>
+           (fun ost min rq rsbTo =>
               (* n <-- getFirstNatMsg; *)
               let n := O in
               (ost +#[implValueIdx <- n]
@@ -400,13 +392,13 @@ Section System.
                   msg_type := MRs;
                   msg_value := VNat n |})).
 
-      Definition liGetSRsDownDownS: Rule ImplOStateIfc :=
+      Definition liGetSRsDownDownS: Rule :=
         rule.rsdd[0~>2~>0]
         :accepts mesiRsS
         :holding mesiRqS
         :requires FirstNatMsg
         :transition
-           (fun (ost: OState ImplOStateIfc) min rq rsbTo =>
+           (fun ost min rq rsbTo =>
               (* n <-- getFirstNatMsg; *)
               let n := O in
               (ost +#[implValueIdx <- n]
@@ -416,13 +408,13 @@ Section System.
                   msg_type := MRs;
                   msg_value := VNat n |})).
 
-      Definition liGetSRsDownDownE: Rule ImplOStateIfc :=
+      Definition liGetSRsDownDownE: Rule :=
         rule.rsdd[0~>2~>1]
         :accepts mesiRsE
         :holding mesiRqS
         :requires FirstNatMsg
         :transition
-           (fun (ost: OState ImplOStateIfc) min rq rsbTo =>
+           (fun ost min rq rsbTo =>
               (* n <-- getFirstNatMsg; *)
               let n := O in
               (ost +#[implDirIdx <- setDirE (objIdxOf rsbTo)],
@@ -431,32 +423,28 @@ Section System.
                   msg_value := VNat n |})).
 
       (* commonly used *)
-      Definition downSImm: Rule ImplOStateIfc :=
+      Definition downSImm: Rule :=
         rule.immu[0~>3]
         :accepts mesiDownRqS
         :me oidx
-        :requires
-           (fun (ost: OState ImplOStateIfc) orq mins =>
-              mesiS <= ost#[implStatusIdx])
+        :requires (fun ost orq mins => mesiS <= ost#[implStatusIdx])
         :transition
-           (fun (ost: OState ImplOStateIfc) min =>
+           (fun ost min =>
               (ost +#[implStatusIdx <- mesiS],
                {| msg_id := mesiDownRsS;
                   msg_type := MRs;
                   msg_value := VNat (ost#[implValueIdx]) |})).
 
-      Definition liGetSRqUpDownME: Rule ImplOStateIfc :=
+      Definition liGetSRqUpDownME: Rule :=
         rule.rqud[cidx~>0~>4~>0]
         :accepts mesiRqS
         :from cidx
         :me oidx
         :requires
-           ((fun (ost: OState ImplOStateIfc) orq mins =>
-               ost#[implStatusIdx] = mesiI) /\
-            (fun (ost: OState ImplOStateIfc) orq mins =>
-               mesiE <= ost#[implDirIdx].(dir_st)))
+           ((fun ost orq mins => ost#[implStatusIdx] = mesiI) /\
+            (fun ost orq mins => mesiE <= ost#[implDirIdx].(dir_st)))
         :transition
-           (fun (ost: OState ImplOStateIfc) msg =>
+           (fun ost msg =>
               ([ost#[implDirIdx].(dir_excl)],
                {| msg_id := mesiDownRqS;
                   msg_type := MRq;
@@ -464,31 +452,29 @@ Section System.
 
       (** TODO: if we pick a representative among sharers to get a clean value,
        * what is the difference between this protocol and MOSI? *)
-      Definition liGetSRqUpDownS: Rule ImplOStateIfc :=
+      Definition liGetSRqUpDownS: Rule :=
         rule.rqud[cidx~>0~>4~>1]
         :accepts mesiRqS
         :from cidx
         :me oidx
         :requires
-           ((fun (ost: OState ImplOStateIfc) orq mins =>
-               ost#[implStatusIdx] = mesiI) /\
-            (fun (ost: OState ImplOStateIfc) orq mins =>
-               ost#[implDirIdx].(dir_st) = mesiS))
+           ((fun ost orq mins => ost#[implStatusIdx] = mesiI) /\
+            (fun ost orq mins => ost#[implDirIdx].(dir_st) = mesiS))
         :transition
-           (fun (ost: OState ImplOStateIfc) msg =>
+           (fun ost msg =>
               let scidx := hd ii (ost#[implDirIdx].(dir_sharers)) in
               ([scidx],
                {| msg_id := mesiDownRqS;
                   msg_type := MRq;
                   msg_value := VUnit |})).
 
-      Definition liDownSRsUpDown: Rule ImplOStateIfc :=
+      Definition liDownSRsUpDown: Rule :=
         rule.rsud[0~>5]
         :accepts mesiDownRsS
         :holding mesiRqS
         :requires FirstNatMsg
         :transition
-           (fun (ost: OState ImplOStateIfc) mins rq rssFrom rsbTo =>
+           (fun ost mins rq rssFrom rsbTo =>
               (* nv <-- getFirstNatMsg; *)
               let nv := O in
               (ost +#[implValueIdx <- nv]
@@ -498,46 +484,42 @@ Section System.
                   msg_type := MRs;
                   msg_value := VNat nv |})).
 
-      Definition liDownSRqDownDownME: Rule ImplOStateIfc :=
+      Definition liDownSRqDownDownME: Rule :=
         rule.rqdd[0~>6~>0]
         :accepts mesiDownRqS
         :me oidx
         :requires
-           ((fun (ost: OState ImplOStateIfc) orq mins =>
-               ost#[implStatusIdx] = mesiI) /\
-            (fun (ost: OState ImplOStateIfc) orq mins =>
-               mesiE <= ost#[implDirIdx].(dir_st)))
+           ((fun ost orq mins => ost#[implStatusIdx] = mesiI) /\
+            (fun ost orq mins => mesiE <= ost#[implDirIdx].(dir_st)))
         :transition
-           (fun (ost: OState ImplOStateIfc) msg =>
+           (fun ost msg =>
               ([ost#[implDirIdx].(dir_excl)],
                {| msg_id := mesiDownRqS;
                   msg_type := MRq;
                   msg_value := VUnit |})).
 
-      Definition liDownSRqDownDownS: Rule ImplOStateIfc :=
+      Definition liDownSRqDownDownS: Rule :=
         rule.rqdd[0~>6~>1]
         :accepts mesiDownRqS
         :me oidx
         :requires
-           ((fun (ost: OState ImplOStateIfc) orq mins =>
-               ost#[implStatusIdx] = mesiI) /\
-            (fun (ost: OState ImplOStateIfc) orq mins =>
-               ost#[implDirIdx].(dir_st) = mesiS))
+           ((fun ost orq mins => ost#[implStatusIdx] = mesiI) /\
+            (fun ost orq mins => ost#[implDirIdx].(dir_st) = mesiS))
         :transition
-           (fun (ost: OState ImplOStateIfc) msg =>
+           (fun ost msg =>
               let cidx := hd ii (ost#[implDirIdx].(dir_sharers)) in
               ([cidx],
                {| msg_id := mesiDownRqS;
                   msg_type := MRq;
                   msg_value := VUnit |})).
 
-      Definition liDownSRsUpUp: Rule ImplOStateIfc :=
+      Definition liDownSRsUpUp: Rule :=
         rule.rsuu[0~>7]
         :accepts mesiDownRsS
         :holding mesiDownRqS
         :requires FirstNatMsg
         :transition
-           (fun (ost: OState ImplOStateIfc) mins rq rssFrom rsbTo =>
+           (fun ost mins rq rssFrom rsbTo =>
               (* n <-- getFirstNatMsg; *)
               let n := O in
               (ost +#[implValueIdx <- n]
@@ -551,16 +533,15 @@ Section System.
 
     Section SetTrs.
 
-      Definition l1GetMImmE: Rule ImplOStateIfc :=
+      Definition l1GetMImmE: Rule :=
         rule.immd[cidx~>1~>0~>0]
         :accepts mesiRqM
         :from cidx
         :requires
            (FirstNatMsg /\
-            (fun (ost: OState ImplOStateIfc) orq mins =>
-               ost#[implStatusIdx] = mesiE))
+            (fun ost orq mins => ost#[implStatusIdx] = mesiE))
         :transition
-           (fun (ost: OState ImplOStateIfc) msg =>
+           (fun ost msg =>
               (* n <-- getFirstNatMsg; *)
               let n := O in
               (ost +#[implStatusIdx <- mesiM]
@@ -569,16 +550,15 @@ Section System.
                   msg_type := MRs;
                   msg_value := VUnit |})).
 
-      Definition l1GetMImmM: Rule ImplOStateIfc :=
+      Definition l1GetMImmM: Rule :=
         rule.immd[cidx~>1~>0~>1]
         :accepts mesiRqM
         :from cidx
         :requires
            (FirstNatMsg /\
-            (fun (ost: OState ImplOStateIfc) orq mins =>
-               ost#[implStatusIdx] = mesiM))
+            (fun ost orq mins => ost#[implStatusIdx] = mesiM))
         :transition
-           (fun (ost: OState ImplOStateIfc) msg =>
+           (fun ost msg =>
               (* n <-- getFirstNatMsg; *)
               let n := O in
               (ost +#[implValueIdx <- n],
@@ -586,15 +566,13 @@ Section System.
                   msg_type := MRs;
                   msg_value := VUnit |})).
 
-      Definition liGetMImm: Rule ImplOStateIfc :=
+      Definition liGetMImm: Rule :=
         rule.immd[cidx~>1~>0]
         :accepts mesiRqM
         :from cidx
-        :requires
-           (fun (ost: OState ImplOStateIfc) orq mins =>
-              mesiE <= ost#[implStatusIdx])
+        :requires (fun ost orq mins => mesiE <= ost#[implStatusIdx])
         :transition
-           (fun (ost: OState ImplOStateIfc) msg =>
+           (fun ost msg =>
               (ost +#[implStatusIdx <- mesiI]
                    +#[implDirIdx <- setDirM cidx],
                {| msg_id := mesiRsM;
@@ -602,27 +580,25 @@ Section System.
                   msg_value := VUnit |})).
 
       (* commonly used *)
-      Definition getMRqUpUp: Rule ImplOStateIfc :=
+      Definition getMRqUpUp: Rule :=
         rule.rquu[cidx~>1~>1]
         :accepts mesiRqM
         :from cidx
         :me oidx
-        :requires
-           (fun (ost: OState ImplOStateIfc) orq mins =>
-              summaryOf ost <= mesiS)
+        :requires (fun ost orq mins => summaryOf ost <= mesiS)
         :transition
-           (fun (ost: OState ImplOStateIfc) msg =>
+           (fun ost msg =>
               {| msg_id := mesiRqM;
                  msg_type := MRq;
                  msg_value := VUnit |}).
 
-      Definition l1GetMRsDownDown: Rule ImplOStateIfc :=
+      Definition l1GetMRsDownDown: Rule :=
         rule.rsdd[1~>2]
         :accepts mesiRsM
         :holding mesiRqM
         :requires (fun _ _ _ => True)
         :transition
-           (fun (ost: OState ImplOStateIfc) min rq rsbTo =>
+           (fun ost min rq rsbTo =>
               (* n <-- getUpLockNatMsg; *)
               let n := O in
               (ost +#[implStatusIdx <- mesiM]
@@ -634,15 +610,13 @@ Section System.
       (* This is the case where it's possible to directly respond a [mesiRsM]
        * message back since there are no internal sharers to invalidate.
        *)
-      Definition liGetMRsDownDownDirI: Rule ImplOStateIfc :=
+      Definition liGetMRsDownDownDirI: Rule :=
         rule.rsdd[1~>3]
         :accepts mesiRsM
         :holding mesiRqM
-        :requires
-           (fun (ost: OState ImplOStateIfc) orq mins =>
-               ost#[implDirIdx].(dir_st) = mesiI)
+        :requires (fun ost orq mins => ost#[implDirIdx].(dir_st) = mesiI)
         :transition
-           (fun (ost: OState ImplOStateIfc) min rq rsbTo =>
+           (fun ost min rq rsbTo =>
               (ost +#[implStatusIdx <- mesiI]
                    +#[implDirIdx <- setDirM (objIdxOf rsbTo)],
                {| msg_id := mesiRsM;
@@ -652,145 +626,133 @@ Section System.
       (* This is the case where internal invalidation is required due to
        * sharers. 
        *)
-      Definition liGetMRsDownRqDownDirS: Rule ImplOStateIfc :=
+      Definition liGetMRsDownRqDownDirS: Rule :=
         rule.rsrq[1~>4]
         :accepts mesiRsM
         :holding mesiRqM
         :requires
-           (fun (ost: OState ImplOStateIfc) orq mins =>
+           (fun ost orq mins =>
               ost#[implDirIdx].(dir_st) = mesiS)
         :transition
-           (fun (ost: OState ImplOStateIfc) rq =>
+           (fun ost rq =>
               (ost#[implDirIdx].(dir_sharers),
                {| msg_id := mesiDownRqI;
                   msg_type := MRq;
                   msg_value := VUnit |})).
 
-      Definition liDownIRsUpDownDirS: Rule ImplOStateIfc :=
+      Definition liDownIRsUpDownDirS: Rule :=
         rule.rsud[1~>5]
         :accepts mesiDownRsI
         :holding mesiRqM
         :requires (fun _ _ _ => True)
         :transition
-           (fun (ost: OState ImplOStateIfc) mins rq rssFrom rsbTo =>
+           (fun ost mins rq rssFrom rsbTo =>
               (ost +#[implStatusIdx <- mesiI]
                    +#[implDirIdx <- setDirM (objIdxOf rsbTo)],
                {| msg_id := mesiRsM;
                   msg_type := MRs;
                   msg_value := VUnit |})).
 
-      Definition liGetMRqUpDownME: Rule ImplOStateIfc :=
+      Definition liGetMRqUpDownME: Rule :=
         rule.rqud[cidx~>1~>6]
         :accepts mesiRqM
         :from cidx
         :me oidx
         :requires
-           ((fun (ost: OState ImplOStateIfc) orq mins =>
-               ost#[implStatusIdx] = mesiI) /\
-            (fun (ost: OState ImplOStateIfc) orq mins =>
-               mesiE <= ost#[implDirIdx].(dir_st)))
+           ((fun ost orq mins => ost#[implStatusIdx] = mesiI) /\
+            (fun ost orq mins => mesiE <= ost#[implDirIdx].(dir_st)))
         :transition
-           (fun (ost: OState ImplOStateIfc) msg =>
+           (fun ost msg =>
               ([ost#[implDirIdx].(dir_excl)],
                {| msg_id := mesiDownRqI;
                   msg_type := MRq;
                   msg_value := VUnit |})).
 
-      Definition liDownIRsUpDownME: Rule ImplOStateIfc :=
+      Definition liDownIRsUpDownME: Rule :=
         rule.rsud[1~>7]
         :accepts mesiDownRsI
         :holding mesiRqM
         :requires (fun _ _ _ => True)
         :transition
-           (fun (ost: OState ImplOStateIfc) mins rq rssFrom rsbTo =>
+           (fun ost mins rq rssFrom rsbTo =>
               (ost +#[implStatusIdx <- mesiI]
                    +#[implDirIdx <- setDirM (objIdxOf rsbTo)],
                {| msg_id := mesiRsM;
                   msg_type := MRs;
                   msg_value := VUnit |})).
 
-      Definition l1DownIImm: Rule ImplOStateIfc :=
+      Definition l1DownIImm: Rule :=
         rule.immu[1~>8]
         :accepts mesiDownRqI
         :me oidx
-        :requires
-           (fun (ost: OState ImplOStateIfc) orq mins =>
-              mesiS <= ost#[implStatusIdx])
+        :requires (fun ost orq mins => mesiS <= ost#[implStatusIdx])
         :transition
-           (fun (ost: OState ImplOStateIfc) min =>
+           (fun ost min =>
               (ost +#[implStatusIdx <- mesiI],
                {| msg_id := mesiDownRsI;
                   msg_type := MRs;
                   msg_value := VUnit |})).
 
-      Definition liDownIImm: Rule ImplOStateIfc :=
+      Definition liDownIImm: Rule :=
         rule.immu[1~>9]
         :accepts mesiDownRqI
         :me oidx
-        :requires
-           (fun (ost: OState ImplOStateIfc) orq mins =>
-              mesiE <= ost#[implStatusIdx])
+        :requires (fun ost orq mins => mesiE <= ost#[implStatusIdx])
         :transition
-           (fun (ost: OState ImplOStateIfc) min =>
+           (fun ost min =>
               (ost +#[implStatusIdx <- mesiI],
                {| msg_id := mesiDownRsI;
                   msg_type := MRs;
                   msg_value := VUnit |})).
 
-      Definition liDownIRqDownDownDirS: Rule ImplOStateIfc :=
+      Definition liDownIRqDownDownDirS: Rule :=
         rule.rqdd[1~>10]
         :accepts mesiDownRqI
         :me oidx
-        :requires
-           (fun (ost: OState ImplOStateIfc) orq mins =>
-              ost#[implDirIdx].(dir_st) = mesiS)
+        :requires (fun ost orq mins => ost#[implDirIdx].(dir_st) = mesiS)
         :transition
-           (fun (ost: OState ImplOStateIfc) msg =>
+           (fun ost msg =>
               (ost#[implDirIdx].(dir_sharers),
                {| msg_id := mesiDownRqI;
                   msg_type := MRq;
                   msg_value := VUnit |})).
 
-      Definition liDownIRqDownDownDirME: Rule ImplOStateIfc :=
+      Definition liDownIRqDownDownDirME: Rule :=
         rule.rqdd[1~>11]
         :accepts mesiDownRqI
         :me oidx
         :requires
-           ((fun (ost: OState ImplOStateIfc) orq mins =>
-               ost#[implStatusIdx] = mesiI) /\
-            (fun (ost: OState ImplOStateIfc) orq mins =>
-               mesiE <= ost#[implDirIdx].(dir_st)))
+           ((fun ost orq mins => ost#[implStatusIdx] = mesiI) /\
+            (fun ost orq mins => mesiE <= ost#[implDirIdx].(dir_st)))
         :transition
-           (fun (ost: OState ImplOStateIfc) msg =>
+           (fun ost msg =>
               ([ost#[implDirIdx].(dir_excl)],
                {| msg_id := mesiDownRqI;
                   msg_type := MRq;
                   msg_value := VUnit |})).
 
-      Definition liDownIRsUpUp: Rule ImplOStateIfc :=
+      Definition liDownIRsUpUp: Rule :=
         rule.rsuu[1~>12]
         :accepts mesiDownRsI
         :holding mesiDownRqI
         :requires (fun _ _ _ => True)
         :transition
-           (fun (ost: OState ImplOStateIfc) mins rq rssFrom rsbTo =>
+           (fun ost mins rq rssFrom rsbTo =>
               (ost +#[implDirIdx <- setDirI],
                {| msg_id := mesiDownRsI;
                   msg_type := MRs;
                   msg_value := VUnit |})).
 
-      Definition memGetMRqUpDownDirS: Rule ImplOStateIfc :=
+      Definition memGetMRqUpDownDirS: Rule :=
         rule.rqud[cidx~>1~>13]
         :accepts mesiRqM
         :from cidx
         :me oidx
         :requires
-           ((fun (ost: OState ImplOStateIfc) orq mins =>
-               ost#[implStatusIdx] <= mesiS) /\
-            (fun (ost: OState ImplOStateIfc) orq mins =>
-               mesiE <= ost#[implDirIdx].(dir_st)))
+           ((fun ost orq mins => ost#[implStatusIdx] <= mesiS) /\
+            (fun ost orq mins => mesiE <= ost#[implDirIdx].(dir_st)))
         :transition
-           (fun (ost: OState ImplOStateIfc) msg =>
+           (fun ost msg =>
               (ost#[implDirIdx].(dir_sharers),
                {| msg_id := mesiDownRqI;
                   msg_type := MRq;
@@ -806,95 +768,84 @@ Section System.
        * written to a new value, i.e., the value is clean.
        *)
 
-      Definition putRqUpUp: Rule ImplOStateIfc :=
+      Definition putRqUpUp: Rule :=
         rule.rqu[2~>0]
         :me oidx
-        :requires
-           (fun (ost: OState ImplOStateIfc) orq mins =>
-              ost#[implStatusIdx] < mesiM)
+        :requires (fun ost orq mins => ost#[implStatusIdx] < mesiM)
         :transition
-           (fun (ost: OState ImplOStateIfc) =>
+           (fun ost =>
               {| msg_id := mesiRqI;
                  msg_type := MRq;
                  msg_value := VUnit |}).
 
-      Definition putRqUpUpM: Rule ImplOStateIfc :=
+      Definition putRqUpUpM: Rule :=
         rule.rqu[2~>1]
         :me oidx
-        :requires
-           (fun (ost: OState ImplOStateIfc) orq mins =>
-              ost#[implStatusIdx] = mesiM)
+        :requires (fun ost orq mins => ost#[implStatusIdx] = mesiM)
         :transition
-           (fun (ost: OState ImplOStateIfc) =>
+           (fun ost =>
               {| msg_id := mesiRqI;
                  msg_type := MRq;
                  msg_value := VNat (ost#[implValueIdx]) |}).
 
-      Definition putRsDownDown: Rule ImplOStateIfc :=
+      Definition putRsDownDown: Rule :=
         rule.rsd[2~>2]
         :accepts mesiRsI
         :holding mesiRqI
         :requires (fun _ _ _ => True)
         :transition
-           (fun (ost: OState ImplOStateIfc) min rq =>
+           (fun ost min rq =>
               ost +#[implStatusIdx <- mesiI]).
 
-      Definition liPutImmI: Rule ImplOStateIfc :=
+      Definition liPutImmI: Rule :=
         rule.immd[cidx~>2~>3]
         :accepts mesiRqI
         :from cidx
-        :requires
-           (fun (ost: OState ImplOStateIfc) orq mins =>
-              getDir cidx ost#[implDirIdx] = mesiI)
+        :requires (fun ost orq mins => getDir cidx ost#[implDirIdx] = mesiI)
         :transition
-           (fun (ost: OState ImplOStateIfc) msg =>
+           (fun ost msg =>
               (ost, {| msg_id := mesiRsI;
                        msg_type := MRs;
                        msg_value := VUnit
                     |})).
 
-      Definition liPutImmS: Rule ImplOStateIfc :=
+      Definition liPutImmS: Rule :=
         rule.immd[cidx~>2~>4]
         :accepts mesiRqI
         :from cidx
-        :requires
-           (fun (ost: OState ImplOStateIfc) orq mins =>
-              getDir cidx ost#[implDirIdx] = mesiS)
+        :requires (fun ost orq mins => getDir cidx ost#[implDirIdx] = mesiS)
         :transition
-           (fun (ost: OState ImplOStateIfc) msg =>
+           (fun ost msg =>
               (ost +#[implDirIdx <- removeSharer cidx ost#[implDirIdx]],
                {| msg_id := mesiRsI;
                   msg_type := MRs;
                   msg_value := VUnit
                |})).
 
-      Definition memPutImmSNotLast: Rule ImplOStateIfc :=
+      Definition memPutImmSNotLast: Rule :=
         rule.immd[cidx~>2~>4~>0]
         :accepts mesiRqI
         :from cidx
         :requires
-           (fun (ost: OState ImplOStateIfc) orq mins =>
-              and (getDir cidx ost#[implDirIdx] = mesiS)
-                  (List.length ost#[implDirIdx].(dir_sharers) >= 2))
+           ((fun ost orq mins => getDir cidx ost#[implDirIdx] = mesiS) /\
+            (fun ost orq mins => List.length ost#[implDirIdx].(dir_sharers) >= 2))
         :transition
-           (fun (ost: OState ImplOStateIfc) msg =>
+           (fun ost msg =>
               (ost +#[implDirIdx <- removeSharer cidx ost#[implDirIdx]],
                {| msg_id := mesiRsI;
                   msg_type := MRs;
                   msg_value := VUnit
                |})).
 
-      Definition memPutImmSLast: Rule ImplOStateIfc :=
+      Definition memPutImmSLast: Rule :=
         rule.immd[cidx~>2~>4~>1]
         :accepts mesiRqI
         :from cidx
         :requires
-           ((fun (ost: OState ImplOStateIfc) orq mins =>
-               getDir cidx ost#[implDirIdx] = mesiS) /\
-            (fun (ost: OState ImplOStateIfc) orq mins =>
-               List.length ost#[implDirIdx].(dir_sharers) = 1))
+           ((fun ost orq mins => getDir cidx ost#[implDirIdx] = mesiS) /\
+            (fun ost orq mins => List.length ost#[implDirIdx].(dir_sharers) = 1))
         :transition
-           (fun (ost: OState ImplOStateIfc) msg =>
+           (fun ost msg =>
               (ost +#[implStatusIdx <- mesiM]
                    +#[implDirIdx <- setDirI],
                {| msg_id := mesiRsI;
@@ -902,15 +853,13 @@ Section System.
                   msg_value := VUnit
                |})).
 
-      Definition liPutImmE: Rule ImplOStateIfc :=
+      Definition liPutImmE: Rule :=
         rule.immd[cidx~>2~>5]
         :accepts mesiRqI
         :from cidx
-        :requires
-           (fun (ost: OState ImplOStateIfc) orq mins =>
-              getDir cidx ost#[implDirIdx] = mesiE)
+        :requires (fun ost orq mins => getDir cidx ost#[implDirIdx] = mesiE)
         :transition
-           (fun (ost: OState ImplOStateIfc) msg =>
+           (fun ost msg =>
               (ost +#[implStatusIdx <- mesiM]
                    +#[implDirIdx <- setDirI],
                {| msg_id := mesiRsI;
@@ -918,16 +867,15 @@ Section System.
                   msg_value := VUnit
                |})).
 
-      Definition liPutImmM: Rule ImplOStateIfc :=
+      Definition liPutImmM: Rule :=
         rule.immd[cidx~>2~>6]
         :accepts mesiRqI
         :from cidx
         :requires
            (FirstNatMsg /\
-            (fun (ost: OState ImplOStateIfc) orq mins =>
-               getDir cidx ost#[implDirIdx] = mesiM))
+            (fun ost orq mins => getDir cidx ost#[implDirIdx] = mesiM))
         :transition
-           (fun (ost: OState ImplOStateIfc) msg =>
+           (fun ost msg =>
               (* n <-- getFirstNatMsg; *)
               let n := O in
               (ost +#[implStatusIdx <- mesiM]
@@ -948,7 +896,7 @@ Section System.
 
       Local Notation eidx := (l1ExtOf oidx).
 
-      Definition l1: Object ImplOStateIfc :=
+      Definition l1: Object :=
         {| obj_idx := oidx;
            obj_rules :=
              [(** rules involved with [GetS] *)
@@ -964,7 +912,7 @@ Section System.
 
     End L1.
 
-    Definition liRulesFromChild (cidx: IdxT): list (Rule ImplOStateIfc) :=
+    Definition liRulesFromChild (cidx: IdxT): list (Rule) :=
       [liGetSImmS cidx; liGetSImmME cidx; getSRqUpUp oidx cidx;
          liGetSRqUpDownME oidx cidx; liGetSRqUpDownS oidx cidx;
            liGetMImm cidx; getMRqUpUp oidx cidx; liGetMRsDownDownDirI;
@@ -972,10 +920,10 @@ Section System.
              liPutImmI cidx; liPutImmS cidx;
                liPutImmE cidx; liPutImmM cidx].
 
-    Definition liRulesFromChildren (coinds: list IdxT): list (Rule ImplOStateIfc) :=
+    Definition liRulesFromChildren (coinds: list IdxT): list (Rule) :=
       List.concat (map liRulesFromChild coinds).
 
-    Program Definition li: Object ImplOStateIfc :=
+    Program Definition li: Object :=
       {| obj_idx := oidx;
          obj_rules :=
            (liRulesFromChildren (subtreeChildrenIndsOf topo oidx))
@@ -996,7 +944,7 @@ Section System.
     Next Obligation.
     Admitted.
 
-    Definition memRulesFromChild (cidx: IdxT): list (Rule ImplOStateIfc) :=
+    Definition memRulesFromChild (cidx: IdxT): list (Rule) :=
       [liGetSImmS cidx; liGetSImmME cidx;
          liGetSRqUpDownME oidx cidx; liGetSRqUpDownS oidx cidx;
            liGetMImm cidx; liGetMRqUpDownME oidx cidx; memGetMRqUpDownDirS oidx cidx;
@@ -1004,10 +952,10 @@ Section System.
              memPutImmSNotLast cidx; memPutImmSLast cidx;
                liPutImmE cidx; liPutImmM cidx].
 
-    Definition memRulesFromChildren (coinds: list IdxT): list (Rule ImplOStateIfc) :=
+    Definition memRulesFromChildren (coinds: list IdxT): list (Rule) :=
       List.concat (map memRulesFromChild coinds).
              
-    Program Definition mem: Object ImplOStateIfc :=
+    Program Definition mem: Object :=
       {| obj_idx := oidx;
          obj_rules :=
            (memRulesFromChildren (subtreeChildrenIndsOf topo oidx))
@@ -1018,7 +966,7 @@ Section System.
     
   End Objects.
 
-  Program Definition impl: System ImplOStateIfc :=
+  Program Definition impl: System :=
     {| sys_objs :=
          (map li cifc.(c_li_indices)) ++ (map l1 cifc.(c_l1_indices));
        sys_oinds_valid := _;
